theorem_pile.sml
@@ -1,0 +1,16 @@
+val helper_theorem = prove(
+``( ! a . let b = f a in p b )
+ ==>
+ (! a . ? b. (b = f a) /\ p b)``,
+ rw [] >>
+ POP_ASSUM (ASSUME_TAC o EVAL_RULE o SPEC ``a``  ) >>
+ rw [] 
+      );
+
+val helper_theorem_two = prove(
+``(! a . ? b. (b = f a) /\ p b)
+ ==>
+( ! a . let b = f a in p b )
+ ``,
+ simp [] 
+      );
